---
chapterName: "Survey Sampling"
chapter: 7
solution: "51"
order: "051"
date: 2017-10-27 
---

To prove that bias of $$\, \hat \theta_J \,$$ is of the order of $$\, n^{-2} \,$$, we need to show $$\, \Exp(\hat \theta_J) \,$$ contains one term equals to $$\, \theta \,$$ and remaining terms contains $$\, n^{2} \,$$ or higher powers in denominator.

Given:

$$\, \Exp(\hat \theta) = \theta + \frac {b_1} n +  \frac {b_2} {n^2} + \frac {b_3} {n^3} + ... \,$$


$$\, \Exp(\hat \theta_j) = \theta + \frac {b_1} {m(p-1)} +  \frac {b_2} {(m(p-1))^2} + ... \,$$

$$\, V_j = p{\hat \theta} - (p-1){\hat \theta_j} \,$$

$$\, \hat \theta_J = \frac 1 p \sum_{j=1}^{p} V_j \,$$

Proof:

$$\, 
\begin{align*}
\Exp(\hat \theta_J) &= \Exp \Prn{ \frac 1 p \sum_{j=1}^{p} V_j } \\
					&= \Exp \Prn{ \frac 1 p \sum_{j=1}^{p} (p{\hat \theta} - (p-1){\hat \theta_j}) } \\
					&= \frac 1 p\sum_{j=1}^{p} \Exp (p{\hat \theta} - (p-1){\hat \theta_j}) \\
					&= \frac 1 p\sum_{j=1}^{p} \Prn{p\Exp{\hat \theta} - (p-1)\Exp{\hat \theta_j} } \\
					&= \frac 1 p\sum_{j=1}^{p} \Prn{p\Prn{\theta + \frac {b_1} n +  \frac {b_2} {n^2} + ...} - (p-1)\Prn{\theta + \frac {b_1} {m(p-1)} +  \frac {b_2} {(m(p-1))^2} + ...} } \\
					&= \frac 1 p\sum_{j=1}^{p} \Prn{p\Prn{\theta + \frac {b_1} n +  \frac {b_2} {n^2} + ...} - \Prn{(p-1)\theta + \frac {b_1} {m} +  \frac {b_2} {m^2(p-1)^{2-1}} + ...} } \\
					&= \frac 1 p\sum_{j=1}^{p} \Prn{ (p+1-p)\theta + \Prn{\frac p n - \frac 1 m}b_1 + \Prn{\frac p {n^2} - \frac 1 {m^2(p-1)} }b_2 + \Prn{\frac p {n^3} - \frac 1 {m^3(p-1)^2} }b_3 + ...} \\
					&= \frac 1 p\sum_{j=1}^{p} \Prn{\theta + \Prn{\frac p {mp} - \frac 1 m}b_1 + \Prn{\frac {p m^2 (p-1) - n^2} {m^2 n^2 (p-1)} }b_2 + ...} \\
					&= \frac 1 p\sum_{j=1}^{p} \Prn{\theta + 0 + \Prn{\frac {p m^2 (p-1) - m^2 p^2} {m^2 n^2 (p-1)} }b_2 + ...} \\
					&= \frac 1 p\sum_{j=1}^{p} \Prn{\theta + \Prn{\frac {m^2 p} {m^2 n^2 (p-1)} }b_2 + ...} \\
					&= \frac 1 p\sum_{j=1}^{p} \Prn{\theta + \Prn{\frac p {n^2 (p-1)} }b_2 + ...} \\
					&= \theta + \Prn{\frac p {n^2 (p-1)} }b_2 + ... \\
\end{align*}
\,$$

Last step is reduced by removing summation and division by $$\, p \,$$ because every terms occurs $$\, p \,$$ times in the sum.

Thus all the terms contains $$\, n^2 \,$$ or higher powers in the denominator.
